Define Wff mutually with Wt instead of inlining it

typing.v
@@ -22,54 +22,79 @@ Qed.
 Tactic Notation "asimpldep" := repeat (progress ((try (rewrite dep_ith_ren_tm));rewrite /dep_ith; asimpl)).
 
 Inductive Wt (n : nat) (Γ : context) : tm -> tm -> Prop :=
-| T_Var i (UAssn : fin -> nat) :
-  (* This mess is the wff condition *)
-  (* Need to skolemize the existential because otherwise the IH is unusable *)
-  (forall j, j < n -> Wt (n - S j) (Nat.add (S j) >> Γ) (Γ j) (tUniv (UAssn j))) ->
+| T_Var i :
+  Wff n Γ ->
   i < n ->
   (* ------ *)
   Wt n Γ (var_tm i) (dep_ith Γ i)
+
 | T_False i :
+  Wff n Γ ->
   (* -------- *)
   Wt n Γ tFalse (tUniv i)
+
 | T_Pi i A B :
   Wt n Γ A (tUniv i) ->
   Wt (S n) (A .: Γ) B (tUniv i) ->
   (* --------------------- *)
   Wt n Γ (tPi A B) (tUniv i)
+
 | T_Abs A a B i :
-  (* Wt n Γ A (tUniv i) -> *)
   Wt n Γ (tPi A B) (tUniv i) ->
   Wt (S n) (A .: Γ) a B ->
   (* -------------------- *)
   Wt n Γ (tAbs A a) (tPi A B)
+
 | T_App a A B b :
   Wt n Γ a (tPi A B) ->
   Wt n Γ b A ->
   (* -------------------- *)
   Wt n Γ (tApp a b) (subst_tm (b..) B)
+
 | T_Conv a A B i :
   Wt n Γ a A ->
   Wt n Γ B (tUniv i) ->
   Join A B ->
   (* ----------- *)
   Wt n Γ a B
+
 | T_On :
+  Wff n Γ ->
   (* --------- *)
   Wt n Γ tOn tSwitch
+
 | T_Off :
+  Wff n Γ ->
   (* --------- *)
   Wt n Γ tOff tSwitch
+
 | T_If a b c A :
   Wt n Γ a tSwitch ->
   Wt n Γ b A ->
   Wt n Γ c A ->
   (* ------------ *)
   Wt n Γ (tIf a b c) A
+
 | T_Switch i :
+  Wff n Γ ->
   (* ----------- *)
   Wt n Γ tSwitch (tUniv i)
+
 | T_Univ i j :
+  Wff n Γ ->
   i < j ->
   (* ------------ *)
-  Wt n Γ (tUniv i) (tUniv j).
+  Wt n Γ (tUniv i) (tUniv j)
+
+with Wff (n : nat) (Γ : context) : Prop :=
+(* The arithmetic is needed because of the types in the context are scoped differently *)
+(* Need to skolemize the existential as F because otherwise the IH is unusable *)
+| Wff_intro F :
+  (forall i, i < n -> Wt (n - S i) (Nat.add (S i) >> Γ) (Γ i) (tUniv (F i))) ->
+  (* ---------------------------------------------------------------- *)
+  Wff n Γ.
+
+Scheme wt_ind := Induction for Wt Sort Prop
+    with wff_ind := Induction for Wff Sort Prop.
+
+Combined Scheme wt_mutual from wt_ind, wff_ind.
